fstar-helpers/fstar-bitvec/BitVec.Intrinsics.fsti
@@ -3,13 +3,9 @@ module BitVec.Intrinsics
 open Core
 open Rust_primitives
 open FStar.Mul
-
-(*** BitVec related utils *)
-open FStar.FunctionalExtensionality
+open BitVec.Utils
 open BitVec.Equality
-open Rust_primitives.BitVectors
-
-let mk_bv #len (f: (i:nat{i < len}) -> bit) = on (i:nat {i < len}) f
+open Tactics.Utils
 
 (*** The intrinsics *)
 
@@ -27,6 +23,46 @@ let mm256_castsi256_si128 (vec: bit_vec 256): bit_vec 128
   = mk_bv (fun i -> vec i)
 let mm256_extracti128_si256 (control: i32{control == 1l}) (vec: bit_vec 256): bit_vec 128
   = mk_bv (fun i -> vec (i + 128))
+
+let mm256_set_epi16 (x0 x1 x2 x3 x4 x5 x6 x7 x8 x9 x10 x11 x12 x13 x14 x15: i16)
+  : bit_vec 256
+  = mk_bv (fun i ->
+      let offset = i % 16 in
+      match i / 16 with
+      |  0 -> get_bit x15 (sz offset)
+      |  1 -> get_bit x14 (sz offset)
+      |  2 -> get_bit x13 (sz offset)
+      |  3 -> get_bit x12 (sz offset)
+      |  4 -> get_bit x11 (sz offset)
+      |  5 -> get_bit x10 (sz offset)
+      |  6 -> get_bit x9 (sz offset)
+      |  7 -> get_bit x8 (sz offset)
+      |  8 -> get_bit x7 (sz offset)
+      |  9 -> get_bit x6 (sz offset)
+      | 10 -> get_bit x5 (sz offset)
+      | 11 -> get_bit x4 (sz offset)
+      | 12 -> get_bit x3 (sz offset)
+      | 13 -> get_bit x2 (sz offset)
+      | 14 -> get_bit x1 (sz offset)
+      | 15 -> get_bit x0 (sz offset)
+    )
+
+val mm256_set1_epi16_no_semantics: i16 -> bit_vec 256
+let mm256_set1_epi16_pow2_minus_one (n: nat): bit_vec 256
+  = mk_bv (fun i -> if i <= n then 1 else 0)
+
+let mm256_and_si256 (x y: bit_vec 256): bit_vec 256
+  = mk_bv (fun i -> if y i = 0
+                 then 0
+                 else x i
+          )
+
+let mm256_set1_epi16 (constant: i16)
+  (#[Tactics.exact (match unify_app (quote constant) (quote (fun n -> ((1s <<! Int32.int_to_t n <: i16) -! 1s <: i16))) [] with
+     | Some [x] -> `(mm256_set1_epi16_pow2_minus_one (`#x))
+     | _ -> (quote (mm256_set1_epi16_no_semantics constant))
+  )]result: bit_vec 256)
+  : bit_vec 256 = result
 
 private let saturate8 (v: bit_vec 16): bit_vec 8
   = let on_upper_bits (+) (f: (n:nat{n >= 8 && n <= 15}) -> _) 
@@ -60,29 +96,6 @@ let mm_movemask_epi8_bv (a: bit_vec 128): bit_vec 128
 let mm_movemask_epi8 (a: bit_vec 128): i32
   = bit_vec_to_int_t 32 (mk_bv (fun i -> mm_movemask_epi8_bv a i))
 
-let mm256_set_epi16 (x0 x1 x2 x3 x4 x5 x6 x7 x8 x9 x10 x11 x12 x13 x14 x15: i16)
-  : bit_vec 256
-  = mk_bv (fun i ->
-      let offset = i % 16 in
-      match i / 16 with
-      |  0 -> get_bit x15 (sz offset)
-      |  1 -> get_bit x14 (sz offset)
-      |  2 -> get_bit x13 (sz offset)
-      |  3 -> get_bit x12 (sz offset)
-      |  4 -> get_bit x11 (sz offset)
-      |  5 -> get_bit x10 (sz offset)
-      |  6 -> get_bit x9 (sz offset)
-      |  7 -> get_bit x8 (sz offset)
-      |  8 -> get_bit x7 (sz offset)
-      |  9 -> get_bit x6 (sz offset)
-      | 10 -> get_bit x5 (sz offset)
-      | 11 -> get_bit x4 (sz offset)
-      | 12 -> get_bit x3 (sz offset)
-      | 13 -> get_bit x2 (sz offset)
-      | 14 -> get_bit x1 (sz offset)
-      | 15 -> get_bit x0 (sz offset)
-    )
-
 let mm_packs_epi16 (a b: bit_vec 128): bit_vec 128
   = mk_bv (fun i ->
       let nth_block = i / 8 in
@@ -96,24 +109,85 @@ let mm_packs_epi16 (a b: bit_vec 128): bit_vec 128
 
 
 // This is a very specialized version of mm256_mullo_epi16
-let specialized_mm256_mullo_epi16 (a: bit_vec 256): bit_vec 256 =
+let mm256_mullo_epi16_specialized1 (a: bit_vec 256): bit_vec 256 =
   mk_bv (fun i -> 
     let nth_bit = i % 16 in
     let nth_i16 = i / 16 in
     let shift = if nth_i16 >= 8 then 23 - nth_i16 else 15 - nth_i16 in
     if nth_bit >= shift then a (i - shift) else 0
   )
+  
+// This is a very specialized version of mm256_mullo_epi16
+let mm256_mullo_epi16_specialized2 (a: bit_vec 256): bit_vec 256 =
+  mk_bv (fun i -> 
+    let nth_bit = i % 16 in
+    let nth_i16 = i / 16 in
+    let shift = if nth_i16 % 2 = 0 then 4 else 0 in
+    if nth_bit >= shift then a (i - shift) else 0
+  )
 
 // This term will be stuck, we don't know anything about it
 val mm256_mullo_epi16_no_semantics (a count: bit_vec 256): bit_vec 256
 
-let mm256_mullo_epi16 (a count: bit_vec 256): bit_vec 256 =
-  if count `bv_equality` mm256_set_epi16 (1s <<! 8l <: i16) (1s <<! 9l <: i16)
-      (1s <<! 10l <: i16) (1s <<! 11l <: i16) (1s <<! 12l <: i16) (1s <<! 13l <: i16)
-      (1s <<! 14l <: i16) (-32768s) (1s <<! 8l <: i16) (1s <<! 9l <: i16) (1s <<! 10l <: i16)
-      (1s <<! 11l <: i16) (1s <<! 12l <: i16) (1s <<! 13l <: i16) (1s <<! 14l <: i16) (-32768s)
-  then specialized_mm256_mullo_epi16 a
-  else mm256_mullo_epi16_no_semantics a count
+open FStar.Tactics.V2
+
+
+
+let mm256_mullo_epi16
+    (a count: bit_vec 256) 
+    (#[(
+      if match unify_app (quote count) (quote (fun x -> mm256_set_epi16 (1s <<! 8l <: i16) (x <<! 9l <: i16)
+                                                               (1s <<! 10l <: i16) (1s <<! 11l <: i16) (1s <<! 12l <: i16) (1s <<! 13l <: i16)
+                                                               (1s <<! 14l <: i16) (-32768s) (1s <<! 8l <: i16) (1s <<! 9l <: i16) (1s <<! 10l <: i16)
+                                                               (1s <<! 11l <: i16) (1s <<! 12l <: i16) (1s <<! 13l <: i16) (1s <<! 14l <: i16) (-32768s))) [] with
+         | Some [x] -> unquote x = 1s
+         | _ -> false
+      then Tactics.exact (quote (mm256_mullo_epi16_specialized1 a))
+      else if match unify_app (quote count) (quote (fun x -> mm256_set_epi16 (1s <<! 0l <: i16) (x <<! 4l <: i16)
+                                                               (1s <<! 0l <: i16) (1s <<! 4l <: i16) (1s <<! 0l <: i16) (1s <<! 4l <: i16) (1s <<! 0l <: i16)
+                                                               (1s <<! 4l <: i16) (1s <<! 0l <: i16) (1s <<! 4l <: i16) (1s <<! 0l <: i16) (1s <<! 4l <: i16)
+                                                               (1s <<! 0l <: i16) (1s <<! 4l <: i16) (1s <<! 0l <: i16) (1s <<! 4l <: i16))) [] with
+              | Some [x] -> unquote x = 1s
+              | _ -> false
+           then Tactics.exact (quote (mm256_mullo_epi16_specialized2 a))
+           else 
+             Tactics.exact (quote (mm256_mullo_epi16_no_semantics a count))
+    )]result: bit_vec 256): bit_vec 256 = result
+
+let madd_rhs (n: nat {n < 16}) = 
+  mm256_set_epi16 
+    (1s <<! Int32.int_to_t n <: i16) 
+    1s 
+    (1s <<! Int32.int_to_t n <: i16) 
+    1s
+    (1s <<! Int32.int_to_t n <: i16) 
+    1s 
+    (1s <<! Int32.int_to_t n <: i16)
+    1s 
+    (1s <<! Int32.int_to_t n <: i16) 
+    1s 
+    (1s <<! Int32.int_to_t n <: i16) 
+    1s
+    (1s <<! Int32.int_to_t n <: i16) 
+    1s 
+    (1s <<! Int32.int_to_t n <: i16) 
+    1s
+
+val mm256_madd_epi16_no_semantic: bit_vec 256 -> bit_vec 256 -> bit_vec 256
+
+let mm256_madd_epi16_specialized (x: bit_vec 256) (n: nat {n < 16}) =
+  x
+
+let mm256_madd_epi16
+  (x y: bit_vec 256) 
+  (#[(
+    let t = match unify_app (quote y) (quote (fun n -> madd_rhs n)) [delta_only [`%madd_rhs]] with
+    | Some [n] -> `(mm256_madd_epi16_specialized (`@x) (`#n))
+    | _ -> quote (mm256_madd_epi16_no_semantic x y) in
+    exact t
+  )]result: bit_vec 256)
+  : bit_vec 256 
+  = result
 
 open FStar.Stubs.Tactics.V2.Builtins
 open FStar.Stubs.Tactics.V2
